Repair accidentaly changed test file

Test/git-issues/git-issue-1989.dfy
@@ -1,6 +1,27 @@
 // RUN: %exits-with 4 %dafny /compile:0 "%s" > "%t"
 // RUN: %diff "%s.expect" "%t"
 
+// ---------------------------------------
+
+module Test {
+  class C {
+  }
+
+  function arrSet(a: array<C>): set<object>
+    reads a
+  {
+    set i : int | 0 <= i < a.Length :: a[i]
+  }
+
+  method test(a: array<C>, i: int, x: C)
+    modifies a
+    requires 0 <= i < a.Length
+    requires x !in arrSet(a)
+  {
+    a[i] := x;
+    assert arrSet(a) == arrSet(old(a)); // warning: old has no effect
+  }
+}
 
 // ---------------------------------------
 
@@ -8,6 +29,36 @@ predicate P(s: seq<int>)
 predicate Q(a: array<int>)
   reads a
 
+class C {
+  var x: int
+
+  predicate PInClass(s: seq<int>)
+  static predicate StaticPInClass(s: seq<int>)
+
+  predicate QInClass(a: array<int>)
+    reads a
+  static predicate StaticQInClass(a: array<int>)
+    reads a
+
+  predicate R(y: int := x)
+    reads this
+}
+
+method TestsNoReads(c: C, s: seq<int>, a: array<int>) {
+  ghost var b;
+  b := old(P(s)); // warning: old has no effect
+  b := old(c.PInClass(s)); // warning: old has no effect
+  b := old(C.StaticPInClass(s)); // warning: old has no effect
+  b := old(c.StaticPInClass(s)); // warning: old has no effect
+
+  b := old(Q(a));
+  b := old(c.QInClass(a));
+  b := old(C.StaticQInClass(a));
+  b := old(c.StaticQInClass(a));
+
+  b := old(c.R(3));
+  b := old(c.R());
+}
 
 method Trigger()
   // The following should generate a warning, but preferably not two.
@@ -18,4 +69,170 @@ method Trigger()
   // A manually supplied trigger should have its own warning, though:
   ensures forall s {:trigger old(P(s))} :: P(s) == old(P(s)) // warning (x2): old has no effect
 {
+}
+
+// An iterator has several auto-generated old expressions.
+// These should not generate any warnings.
+iterator Iter()
+{
+}
+
+// ---------------------------------------
+
+class D {
+  var data: int
+  const N: int
+  var arr: array<real>
+
+  method TestFields()
+    ensures data == old(data)
+    ensures N == old(N) // warning: old has no effect, since N is const
+  {
+  }
+
+  method TestArrayElements(j: nat, a: array<real>)
+    requires j < a.Length
+    ensures a.Length == old(a.Length) // warning: old has no effect
+    ensures a[j] == old(a[j])
+    ensures a[j] == old(a)[j] // warning: old has no effect
+    ensures a[j] == a[old(j)] // warning: old has no effect
+  {
+  }
+
+  method MoreArrays(b: array<real>)
+    requires 0 <= data && data + 1 < arr.Length == b.Length
+    requires 1.0 <= arr[data] < arr[data + 1] < 2.0
+    requires 4.0 <= b[data] < b[data + 1] < 5.0
+    modifies this, arr
+    ensures arr == b && data == old(data) + 1
+    ensures arr[data] != old(arr[data])
+    ensures arr[data] != old(arr)[data]
+    ensures arr[data] != arr[old(data)]
+    ensures var a, j := arr, data; old(arr[data]) != old(a[j])
+  {
+    forall i | 0 <= i < arr.Length {
+      arr[i] := 2.0 * arr[i];
+    }
+    arr := b;
+    data := data + 1;
+  }
+
+  method TestMatrixElements(i: nat, j: nat, m: array2<real>)
+    requires i < m.Length0 && j < m.Length1
+    ensures m.Length0 == old(m.Length1) // warning: old has no effect
+    ensures m[i, j] == old(m[i, j])
+    ensures m[i, j] == old(m)[i, j] // warning: old has no effect
+    ensures m[i, j] == m[i, old(j)] // warning: old has no effect
+  {
+  }
+
+  lemma Lemma(y: int)
+    requires data == y
+  {
+  }
+}
+
+
+lemma StaticLemmaWithoutPrecondition(y: int)
+{
+}
+
+// ---------------------------------------
+
+method StmtExpr(d: D)
+  requires d.data == 3
+  modifies d
+{
+  ghost var a;
+  d.data := 100;
+  if {
+  case true =>
+    a := assert d.data < 5; 10; // error: assertion failure
+  case true =>
+    a := old(20 + assert d.data < 5; 10);
+  case true =>
+    a := old(d.Lemma(3); 10);
+  case true =>
+    a := old(d.Lemma(100); 10); // error: precondition violation
+  case true =>
+    a := (d.Lemma(old(100)); 10); // warning: old has no effect
+  }
+  a := assert d.data < old(105); 0; // warning: old has no effect
+}
+
+method CalcStmtExpr(d: D)
+  requires d.data == 3
+  modifies d
+{
+  ghost var a;
+  d.data := 100;
+  if {
+  case true =>
+    a := old(calc { } 10); // warning: old has no effect
+  case true =>
+    a := old(calc {
+      2;
+    ==  { assert d.data == 3; }
+      2;
+    } 10);
+  case true =>
+    a := old(calc {
+      2;
+    ==  { assert d.data == 100; } // error: assertion violation
+      2;
+    } 10);
+  case true =>
+    a := old(calc {
+      2;
+    ==  { d.Lemma(3); }
+      2;
+    } 10);
+  case true =>
+    a := old(calc {
+      2;
+    ==  { StaticLemmaWithoutPrecondition(3); }
+      2;
+    } 10);
+  case true =>
+    a := old(calc {
+      2;
+    ==  { d.Lemma(100); } // error: precondition violation
+      2;
+    } 10);
+  }
+}
+
+twostate function CalcStmtExprFunction(d: D, selector: int): int
+  requires old(d.data) == 3 && d.data == 100
+  reads d
+{
+  match selector
+  case 0 =>
+    old(calc { } 10) // warning: old has no effect
+  case 1 =>
+    old(calc {
+      2;
+    ==  { assert d.data == 3; }
+      2;
+    } 10)
+  case 2 =>
+    old(calc {
+      2;
+    ==  { assert d.data == 100; } // error: assertion violation
+      2;
+    } 10)
+  case 3 =>
+    old(calc {
+      2;
+    ==  { d.Lemma(3); }
+      2;
+    } 10)
+  case 4 =>
+    old(calc {
+      2;
+    ==  { d.Lemma(100); } // error: precondition violation
+      2;
+    } 10)
+  case _ =>
+    10
 }
